MyOCL.thy
@@ -24,19 +24,26 @@ datatype OCLexp = Int nat
   | CollectPlus OCLexp OCLexp OCLexp 
   | PEAtt OCLexp
   | PEAs OCLexp "Enrollment list"
+  | PEVar var "Person list"
   | AllInstances entity
 
-(* COMMENT
 fun partialEval :: "OCLexp \<Rightarrow> Objectmodel \<Rightarrow> OCLexp" where
 "partialEval (MyOCL.Int i) om = (MyOCL.Int i)"
-| "partialEval (MyOCL.Var x) om = (MyOCL.Var x)"
-| "partialEval (MyOCL.IVar i) om = (MyOCL.IVar i)"
 | "partialEval (MyOCL.Eq e1 e2) om = MyOCL.Eq (partialEval e1 om) (partialEval e2 om)" 
-| "partialEval (MyOCL.Att (Var v) att) om = (PEAtt (MyOCL.Att (Var v) att))"
+| "partialEval (MyOCL.IVar i) om = (MyOCL.IVar i)"
+| "partialEval (MyOCL.Var x) om = PEVar x (getPersonList om)"
 | "partialEval (MyOCL.Att (IVar v) att) om = (PEAtt (MyOCL.Att (IVar v) att))"
+(*
+| "partialEval (MyOCL.Var x) om = (getAssignedPerson x (getPersonList om))"
+*)
+(*
+
+| "partialEval (MyOCL.Att (Var v) att) om = (PEAtt (MyOCL.Att (Var v) att))"
 | "partialEval (MyOCL.As (Var v) as) om = (PEAs (MyOCL.As (Var v) as) (getEnrollmentList om))"
 | "partialEval (MyOCL.As (IVar v) as) om = (PEAs (MyOCL.As (IVar v) as) (getEnrollmentList om))"
+*)
 
+(* COMMENT
 fun flatten :: "val \<Rightarrow> val list" where
 "flatten (VList vs) = vs" 
 
@@ -60,7 +67,6 @@ fun projValAs :: "as \<Rightarrow> val \<Rightarrow> Enrollment list \<Rightarro
 (if (getAssociationEnd STUDENTS e) = p
 then ((VPerson (getAssociationEnd LECTURERS e))#(projValAs LECTURERS (VPerson p) es))
 else (projValAs LECTURERS (VPerson p) es))"
-
 
 (*
 "projValAs LECTURERS (VPerson p) [] = []"
